define ifc_funspec as a VST funspec + pre/post heap/stack classifications and define ifc_body similarly to semax_body, so that in the examples, VST has all the context it needs

examples/write_labeled_val_verif.v
@@ -42,7 +42,74 @@ Record MyMetaVars: Type := { v: int; b: int; highptr: val; lowptr: val }.
 
 Set Printing Projections. (* to get x.(b) instead of (b x) in output *)
 
+Definition write_labeled_val_spec: ifc_funspec := {|
+  functional_spec :=
+    DECLARE _write_labeled_val
+    WITH x: MyMetaVars
+    PRE [ _v OF tint, _b OF tbool, _highptr OF (tptr tint), _lowptr OF (tptr tint) ]
+     (PROP (x.(b) = Int.zero \/ x.(b) = Int.one)
+      LOCAL (
+        temp _v (Vint x.(v)); temp _b (Vint x.(b)); temp _highptr x.(highptr); temp _lowptr x.(lowptr)
+      )
+      SEP (data_at_ Ews tint x.(highptr); data_at_ Ews tint x.(lowptr)))
+    POST [ tvoid ]
+      (PROP (x.(b) = Int.zero \/ x.(b) = Int.one)
+       LOCAL (
+         temp _v (Vint x.(v)); temp _b (Vint x.(b)); temp _highptr x.(highptr); temp _lowptr x.(lowptr)
+       )
+       SEP (data_at_ Ews tint x.(highptr); data_at_ Ews tint x.(lowptr)));
+  ifc_stack_pre :=
+    (fun (x: MyMetaVars) (i: ident) => PMap.get i 
+      (PMap.set _v (if Int.eq x.(b) Int.zero then Lo else Hi)
+      (PMap.set _b Lo
+      (PMap.set _highptr Hi
+      (PMap.set _lowptr Lo
+      (PMap.init Hi))))));
+  ifc_heap_pre :=
+    (fun (x: MyMetaVars) (loc: heap_loc) => Hi);
+  ifc_stack_post :=
+    (fun (x: MyMetaVars) (i: ident) => Hi);
+  ifc_heap_post :=
+    (fun (x: MyMetaVars) (loc: heap_loc) => Hi)
+|}.
+
+Definition Gprog: funspecs := [].
+
 Lemma verif_write_labeled_val:
+  ifc_body Vprog Gprog f_write_labeled_val write_labeled_val_spec.
+Proof.
+  unfold write_labeled_val_spec. hnf. intros. clear ts.
+  simpl (fn_body _).
+  (* TODO rule for Ssequence *)
+  replace (Ssequence
+   (Sifthenelse (Etempvar _b tbool)
+      (Sassign (Ederef (Etempvar _highptr (tptr tint)) tint)
+         (Etempvar _v tint))
+      (Sassign (Ederef (Etempvar _lowptr (tptr tint)) tint)
+         (Etempvar _v tint))) (Sreturn None))
+  with (Sifthenelse (Etempvar _b tbool)
+      (Sassign (Ederef (Etempvar _highptr (tptr tint)) tint)
+         (Etempvar _v tint))
+      (Sassign (Ederef (Etempvar _lowptr (tptr tint)) tint)
+         (Etempvar _v tint))) by admit.
+  apply ifc_ifthenelse; try reflexivity; unfold iand, iprop.
+  - (* then-branch *)
+    unfold ifc_def. split.
+    + (* VST part *)
+      intros. destruct x as [v b highptr lowptr] eqn: E.
+      match goal with
+      | _ : x = ?m |- _ => simpl (_ m)
+      end. clear E.
+      simplify_func_tycontext. abbreviate_semax.
+      (* forward. still fails *)
+      admit.
+    + (* IFC part *)
+      apply ifc_core0_always_holds.
+  - (* else-branch *)
+    admit.
+Admitted.
+
+Lemma verif_write_labeled_val_body_only:
   ifc [x: MyMetaVars] Delta |--
    (PROP (x.(b) = Int.zero \/ x.(b) = Int.one)
     LOCAL (
