ifc/ifc.v
@@ -118,3 +118,83 @@ Instance Espec: OracleKind. Admitted.
 Definition t1 := ifc [ a : nat ] D1 |-- P1 N1 A1 Sskip (fun _ => fun _ => !! (a = a)) N1 A1.
 Print t1.
 *)
+
+Definition WITHclause_type(fspec: ident * funspec): Type := match fspec with
+| (_, mk_funspec _ _ (rmaps.ConstType A) _ _ _ _) => A
+(* error: we always expect an rmaps.ConstType, because that's what NDmk_funspec passes to mk_funspec *)
+| _ => unit
+end.
+
+Record ifc_funspec: Type := mk_ifc_funspec {
+  functional_spec : (ident * funspec)%type;
+  ifc_stack_pre   : (WITHclause_type functional_spec) -> stack_clsf;
+  ifc_heap_pre    : (WITHclause_type functional_spec) -> heap_clsf;
+  ifc_stack_post  : (WITHclause_type functional_spec) -> stack_clsf;
+  ifc_heap_post   : (WITHclause_type functional_spec) -> heap_clsf
+}.
+
+Local Open Scope logic.
+
+Require Import veric.rmaps.
+
+(* "T -> assertion" *)
+Definition vst_fun_assert (T: Type): Type :=
+  forall ts : list Type,
+    msl.functors.MixVariantFunctor._functor 
+     (dependent_type_functor_rec ts (AssertTT (rmaps.ConstType T))) mpred.
+
+(* inspired by semax_body in VST/veric/semax_prog.v *)
+Definition ifc_body00 (V: varspecs) (G: funspecs) (C: compspecs) (f: function)
+  (T: Type)
+  (P : vst_fun_assert T) (N : T -> stack_clsf) (A : T -> heap_clsf)
+  (P': vst_fun_assert T) (N': T -> stack_clsf) (A': T -> heap_clsf)
+: Prop :=
+  forall Espec ts,
+    @ifc_def T C Espec (func_tycontext f V G)
+             (fun x rho => P ts x rho * stackframe_of f rho)
+             N A
+             (Ssequence f.(fn_body) (Sreturn None))
+             (fun x => (frame_ret_assert (function_body_ret_assert (fn_return f) (P' ts x))
+                                         (stackframe_of f)))
+             N' A'.
+
+Definition force_const_type(t: TypeTree): Type :=
+      match t with
+      | ConstType A0 => A0
+      | Mpred => unit
+      | DependentType _ => unit
+      | ProdType _ _ => unit
+      | ArrowType _ _ => unit
+      end.
+
+(* dependent types craziness... *)
+Definition ifc_body0 (V : varspecs) (G : funspecs) (C : compspecs) (f : function) (i : ident)
+  (fsig : base.funsig) (c : calling_convention) (T0 : TypeTree)
+  (P P' : forall ts : list Type,
+        functors.MixVariantFunctor._functor
+          (dependent_type_functor_rec ts (AssertTT T0)) mpred)
+  (P_ne : super_non_expansive P) (Q_ne : super_non_expansive P')
+  (N  : WITHclause_type (i, mk_funspec fsig c T0 P P' P_ne Q_ne) -> stack_clsf)
+  (A  : WITHclause_type (i, mk_funspec fsig c T0 P P' P_ne Q_ne) -> heap_clsf)
+  (N' : WITHclause_type (i, mk_funspec fsig c T0 P P' P_ne Q_ne) -> stack_clsf)
+  (A' : WITHclause_type (i, mk_funspec fsig c T0 P P' P_ne Q_ne) -> heap_clsf)
+: Prop := 
+  match T0 as t return
+    (let T := force_const_type t in (forall
+       P0 P'0 ,
+     super_non_expansive P0 ->
+     super_non_expansive P'0 ->
+     (T -> stack_clsf) ->
+     (T -> heap_clsf) ->
+     (T -> stack_clsf) ->
+     (T -> heap_clsf) -> Prop))
+  with
+  | ConstType T => fun P0 P'0 _ _ N0 A0 N'0 A'0 => ifc_body00 V G C f T P0 N0 A0 P'0 N'0 A'0
+  | _ => fun _ _ _ _ _ _ _ _  => False
+  end P P' P_ne Q_ne N A N' A'.
+
+Definition ifc_body
+       (V: varspecs) (G: funspecs) {C: compspecs} (f: function) (spec: ifc_funspec) : Prop :=
+  match spec with (mk_ifc_funspec (i, mk_funspec fsig cc T P P' Pne P'ne) N A N' A') =>
+    ifc_body0 V G C f i fsig cc T P P' Pne P'ne N A N' A'
+  end.
